\documentclass[10pt,a4paper, margin=1in]{article}
\usepackage{fullpage}
\usepackage{amsfonts, amsmath, pifont}
\usepackage{amsthm}
\usepackage{graphicx}
\usepackage{float}


\usepackage{tkz-euclide}
\usepackage{tikz}
\usepackage{pgfplots}
\pgfplotsset{compat=1.13}

\newcommand\ddfrac[2]{\frac{\displaystyle #1}{\displaystyle #2}}

\usepackage{geometry}
 \geometry{
 a4paper,
 total={210mm,297mm},
 left=10mm,
 right=10mm,
 top=10mm,
 bottom=10mm,
 }
 % Write both of your names here. Fill exxxxxxx with your ceng mail address.
 \author{
  Çavuşoğlu, Arda\\
  \texttt{e2448249@ceng.metu.edu.tr}
  \and
  Çolak, Ahmet Eren\\
  \texttt{e2587921@ceng.metu.edu.tr}
}

\title{CENG 384 - Signals and Systems for Computer Engineers \\
Spring 2023 \\
Homework 4}
\begin{document}
\maketitle



\noindent\rule{19cm}{1.2pt}

\begin{enumerate}

\item %write the solution of q1
	\begin{enumerate}   
    % Write your solutions in the following items.
    
    \item %write the solution of q1a
    $H(j\omega) = \frac{Y(j\omega)}{X(j\omega)} = \frac{j\omega-1}{j\omega+1}$ \vspace{0.2cm}\\
    $Y(j\omega)(j\omega+1) = X(j\omega)(j\omega-1)$ \vspace{0.2cm}\\
    $j\omega Y(j\omega)+Y(j\omega) = j\omega X(j\omega)-X(j\omega)$ \vspace{0.2cm}\\
    $\frac{dy(t)}{dt} + y(t) = \frac{dx(t)}{dt} - x(t)$ \vspace{0.2cm}\\
    
    \item %write the solution of q1b
    $H(j\omega) = \frac{j\omega}{j\omega+1}-\frac{1}{j\omega+1} = j\omega \frac{1}{j\omega+1} - \frac{1}{j\omega+1}$ \vspace{0.2cm}\\
    From linearity and differentiation in time properties,\vspace{0.2cm}\\
    $h(t) = \frac{d(e^{-t}u(t))}{dt}-e^{-t}u(t) = -2e^{-t}u(t)$ \vspace{0.2cm}\\
    
    \item %write the solution of q1c
    $x(t) = e^{-2t}u(t) \longleftrightarrow X(j\omega) = \frac{1}{j\omega+2}$ \vspace{0.2cm}\\
    $Y(j\omega) = X(j\omega)H(j\omega) = \frac{j\omega-1}{(j\omega+1)(j\omega+2)} = \frac{3}{j\omega+2} - \frac{2}{j\omega+1}$ \vspace{0.2cm}\\
    $y(t) = 3e^{-2t}u(t) - 2e^{-t}u(t)$ \vspace{0.2cm}\\
    
    \item %write the solution of q1d
    \begin{center}
	\tikzset{%
		block/.style    = {draw, thick, rectangle, minimum height = 3em,
			minimum width = 3em},
		sum/.style      = {draw, circle, node distance = 2cm}, % Adder
		input/.style    = {coordinate}, % Input
		output/.style   = {coordinate} % Output
	}
	% Defining string as labels of certain blocks.
	\newcommand{\suma}{\Large$+$}
	\newcommand{\inte}{$\displaystyle \int$}
	\newcommand{\derv}{\huge$\frac{d}{dt}$}
	
	\begin{tikzpicture}[auto, thick, node distance=2cm, >=triangle 45]
	\draw
	% Drawing the blocks of first filter :
	node at (0, 0) [input] (inp) {\Large \textopenbullet}
        node [output, right of=inp] (temp) {}
	node [output, above of=temp] (temp1) {}
	node [block, right of=temp1] (int1) {\inte}
        node [sum, right of=temp] (sum1) {\suma}
        node [sum, right of=sum1] (sum2) {\suma}
        node [output, right of=int1] (temp2) {}
        node [output, right of=sum2] (out) {}
        node [output, below of=out] (temp4) {}
        node [block, left of=temp4] (int2) {\inte}
        node [output, left of=int2] (temp5) {}
        node [output, right of=out] (out2) {\Large \textopenbullet}
        
	;
	\draw[-](inp) -- node{$x(t)$} (temp);
        \draw[-](temp) -- (temp1);
        \draw[->](temp1) -- (int1);
        \draw[-](inp) -- (temp);
        \draw[->](temp) -- (sum1);
        \draw[->](sum1) -- (sum2);
        \draw[-](int1) -- (temp2);
        \draw[->](temp2) -- node{$-$} (sum2);
        \draw[-](sum2) -- (out);
        \draw[->](out) -- node{y(t)}(out2);
        \draw[-](out) -- (temp4);
        \draw[->](temp4) -- (int2);
        \draw[-](int2) -- (temp5);
        \draw[->](temp5) -- node{$-$} (sum1);

	\end{tikzpicture}
    \end{center} \vspace*{0.2cm}
    
    \end{enumerate}

\vspace*{2cm}
\item %write the solution of q2  
    \begin{enumerate}
    % Write your solutions in the following items.
    \item %write the solution of q2a
    $Y(e^{j\omega})(e^{j\omega}-\frac{1}{2}) = X(e^{j\omega})e^{j\omega}$ \vspace{0.2cm}\\
    $x[n] = \delta[n] \longleftrightarrow X(e^{j\omega}) = 1$ \vspace{0.2cm}\\
    $H(e^{j\omega})(e^{j\omega}-\frac{1}{2}) = e^{j\omega}$ \vspace{0.2cm}\\
    $H(e^{j\omega}) = \frac{e^{j\omega}}{e^{j\omega}-\frac{1}{2}}$
    
    \item %write the solution of q2b
    $H(e^{j\omega}) = \frac{e^{j\omega}}{e^{j\omega}-\frac{1}{2}} = \frac{e^{-j\omega}(e^{j\omega})}{e^{-j\omega}(e^{j\omega}-\frac{1}{2})} = \frac{1}{1-\frac{1}{2}e^{-j\omega}}$ \vspace{0.2cm}\\
    From table, $h[n] = (\frac{1}{2})^n u[n]$ \vspace{0.2cm}\\
    
    \item %write the solution of q2c
    $x[n] = (\frac{3}{4})^n u[n] \longleftrightarrow X(e^{j\omega}) = \frac{1}{1-\frac{3}{4}e^{-j\omega}}$ \vspace{0.2cm}\\
    $Y(e^{j\omega}) = X(e^{j\omega})H(e^{j\omega}) = \frac{1}{1-\frac{1}{2}e^{-j\omega}}\cdot \frac{1}{1-\frac{3}{4}e^{-j\omega}}$ \vspace{0.2cm}\\
    \hspace*{3.8cm}$= \frac{-2}{1-\frac{1}{2}e^{-j\omega}} + \frac{3}{1-\frac{3}{4}e^{-j\omega}}$ \vspace{0.2cm}\\
    From table and linearity property, $y[n] = (3(\frac{3}{4})^n-2(\frac{1}{2})^n)u[n]$
    \end{enumerate}

\item %write the solution of q3
    \begin{enumerate}
    % Write your solutions in the following items.
    \item %write the solution of q3a
    \vspace*{2cm}
    \tikzset{%
        block/.style    = {draw, thick, rectangle, minimum height = 3em,
            minimum width = 3em},
        sum/.style      = {draw, circle, node distance = 2cm}, % Adder
        input/.style    = {coordinate}, % Input
        output/.style   = {coordinate} % Output
    }
    % Defining string as labels of certain blocks.
    \newcommand{\suma}{\Large$+$}
    \newcommand{\inte}{$\displaystyle \int$}
    \newcommand{\derv}{\huge$\frac{d}{dt}$}
    
    \begin{tikzpicture}[auto, thick, node distance=2cm, >=triangle 45]
    \draw
    % Drawing the blocks of first filter :
    node at (0, 0) [input] (inp) {\Large \textopenbullet}
        node [block, right of=inp] (resp1) {$H_1(j\omega)$}
    node [block, right of=resp1] (resp2) {$H_2(j\omega)$}
        node [output, right of=resp2] (out) {\Large \textopenbullet}
        
    ;
    \draw[->](inp) -- node{$x(t)$} (resp1);
        \draw[->](resp1) -- (resp2);
        \draw[->](resp2) -- node{$y(t)$} (out);
    
    \end{tikzpicture} \vspace{0.2cm}\\
    
    Means, \vspace{0.2cm}\\
    
    \begin{tikzpicture}[auto, thick, node distance=2cm, >=triangle 45]
    \draw
    % Drawing the blocks of first filter :
    node at (0, 0) [input] (inp) {\Large \textopenbullet}
    node [block, right of=inp] (resp1) {$H_1(j\omega)H_2(j\omega)$}
    node [output, right of=resp1] (out) {\Large \textopenbullet}
        
    ;
    \draw[->](inp) -- node{$x(t)$} (resp1);
        \draw[->](resp1) -- node{$y(t)$} (out);
    
    \end{tikzpicture} \vspace{0.2cm}\\
    
    $H(j\omega) = H_1(j\omega)H_2(j\omega) = \frac{1}{(j\omega+1)(j\omega+2)} = \frac{1}{(j\omega)^2 + 3j\omega + 2} = \frac{Y(j\omega)}{X(j\omega)}$ \vspace{0.2cm}\\
    $Y(j\omega)((j\omega)^2 + 3j\omega + 2) = X(j\omega)$ \vspace{0.2cm}\\
    $\frac{d^2y(t)}{dt} + 3\frac{dy(t)}{dt} + 2y(t) = x(t)$ \vspace{0.2cm}\\
    
    \item %write the solution of q3b
    $H(j\omega) = H_1(j\omega)H_2(j\omega) = \frac{1}{(j\omega+1)(j\omega+2)} = \frac{1}{j\omega+1} - \frac{1}{j\omega+2}$ \vspace{0.2cm}\\
    From table, $h(t) = (e^{-t}-e^{-2t})u(t)$ \vspace{0.2cm}\\
    
    \item %write the solution of q3c
    $Y(j\omega) = X(j\omega)H(j\omega)$ \vspace{0.2cm}\\
    \hspace*{1.05cm}$= j\omega\frac{1}{j\omega+1} - j\omega\frac{1}{j\omega+2}$ \vspace{0.2cm}\\
    From linearity and differentiation in time properties, \vspace{0.2cm}\\
    $y(t) = \frac{d(e^{-t}u(t))}{dt} - \frac{d(e^{-2t}u(t))}{dt}$ \vspace{0.2cm}\\
    $y(t) = (-e^{-t}+2e^{-2t})u(t)$ \vspace{0.2cm}\\
    \end{enumerate}

\item %write the solution of q4
    \begin{enumerate}   
    % Write your solutions in the following items.
    \item %write the solution of q4
        \begin{equation*}
            H(e^{jw}) = H_1(e^{jw}) + H_2(e^{jw})
        \end{equation*}

        \begin{equation*}
            H(e^{jw}) = \ddfrac{6 + 4.5e^{-jw}}{3+4.5e^{-jw} + 1.5e^{-jw}}
        \end{equation*}

        \begin{equation*}
            \sum_k a_k Y(e^{jw}) e^{-jwk} = \sum_k b_k X(e^{jw})e^{-jwk}
        \end{equation*}

        \begin{equation*}
            H(e^{jw}) = \ddfrac{ Y(e^{jw})}{X(e^{jw})} = \ddfrac{\sum_k a_k e^{-jwk}}{\sum_k b_k e^{-jwk}}
        \end{equation*}

        \begin{equation*}
            3y[n] + 4.5y[n-1]+1.5y[n-2] = 6x[n] + 4.5x[n-1]
        \end{equation*}
    \item %write the solution of q4b
        \begin{equation*}
            H(e^{jw}) = H_1(e^{jw}) + H_2(e^{jw})
        \end{equation*}

        \begin{equation*}
            H(e^{jw}) = \ddfrac{6 + 4.5e^{-jw}}{3+4.5e^{-jw} + 1.5e^{-jw}}
        \end{equation*}
    \item %write the solution of q4c
        \begin{equation*}
            h[n] = \mathcal{F}^{-1} \{ H_1(e^{jw})\} + \mathcal{F}^{-1} \{ H_2(e^{jw})\}
        \end{equation*}

        Using the look-up tables:
        \begin{equation*}
            h[n] = \left ( \ddfrac{-1}{3} \right )^n u[n] +  \left ( \ddfrac{-1}{2} \right )^n u[n] 
        \end{equation*}
    \end{enumerate}

\item %write the solution of q5
    
\end{enumerate}


\end{document}


