\documentclass[11pt]{article}
\usepackage[utf8]{inputenc}
\usepackage[dvips]{graphicx}
\usepackage{fancybox}
\usepackage{verbatim}
\usepackage{array}
\usepackage{latexsym}
\usepackage{alltt}
\usepackage{hyperref}
\usepackage{textcomp}
\usepackage{color}
\usepackage{amsmath}
\usepackage{amsfonts}
\usepackage{tikz}
\usepackage{fitch}  % to use fitch
\usepackage{float}
\usepackage[hmargin=3cm,vmargin=5.0cm]{geometry}
%\topmargin=0cm
\topmargin=-2cm
\addtolength{\textheight}{6.5cm}
\addtolength{\textwidth}{2.0cm}
%\setlength{\leftmargin}{-5cm}
\setlength{\oddsidemargin}{0.0cm}
\setlength{\evensidemargin}{0.0cm}


\begin{document}

\section*{Student Information } 
%Write your full name and id number between the colon and newline
%Put one empty space character after colon and before newline
Full Name :  Ahmet Eren {\c C}olak \newline
Id Number :  2587921 


% ND example using fitch
% delete or comment if you intend to use this to generate the vector pdf 
\section*{Example ND Proof}

Assume that you are asked to prove the following statement using natural deduction for propositional logic.
\\
\begin{equation*}
p \wedge \neg q \rightarrow r, \neg r, p \vdash q.
\end{equation*}


\begin{center}
	\begin{fitchproof}
		\fitchline{$p \wedge \neg q \rightarrow r$}{premise}
		\fitchline{$\neg r$}{premise}
		\fitchline{$p$}{premise}
		\subproof{
			\fitchline{$\neg q$}{assumption}
			\fitchline{$p \wedge \neg q$}{$\wedge i$ 3,4}
			\fitchline{$r$}{$\rightarrow e$ 1,5}
			\fitchline{$\bot$}{$\neg e$ 6,2}
		}
		\fitchline{$\neg \neg q$}{$\neg i$ 4--7}
		\fitchline{$q$}{$\neg \neg e$ 8}
	\end{fitchproof}
\end{center}
\noindent
\newline
% Write your answers below the section tags
\section*{Q. 1}
\begingroup
\fontsize{10pt}{11pt}
\begin{center}
	\begin{align*}
		\neg (p \wedge q) \leftrightarrow (\neg q \rightarrow p) &\equiv (\neg (p \wedge q) \rightarrow (\neg q \rightarrow p)) \wedge ((\neg q \rightarrow p) \rightarrow \neg (p \wedge q)) && \text{by logical equivalency for $\leftrightarrow$}\\
		&\equiv (\neg \neg (p \wedge q) \vee (\neg \neg q \vee p)) \wedge (\neg (\neg \neg q \vee p) \vee \neg (p \wedge q)) && \text{by logical equivalency for $\rightarrow$}\\
		&\equiv ((p \wedge q) \vee (q \vee p)) \wedge (\neg (q \vee p) \vee \neg (p \wedge q)) && \text{by double negation law}\\
		&\equiv ((p \wedge q) \vee (q \vee p)) \wedge \neg((q \vee p) \wedge (p \wedge q)) && \text{by the first De Morgan law}\\
		&\equiv ((q \vee p \vee p) \wedge (q \vee p \vee q)) \wedge \neg((p \wedge q \wedge q) \vee (p \wedge q \wedge p)) && \text{by distributive law}\\
		&\equiv ((q \vee (p \vee p)) \wedge ((q \vee q) \vee p)) \wedge \neg((p \wedge (q \wedge q)) \vee ((p \wedge p) \wedge q)) && \text{by associative and commutative laws}\\
		&\equiv ((q \vee p)) \wedge (q \vee p)) \wedge \neg((p \wedge q) \vee (p \wedge q)) && \text{by idempotent law}\\
		&\equiv (q \vee p) \wedge \neg (p \wedge q) && \text{by idempotent law}
		&\equiv (q \vee p) \wedge (\neg p \vee \neg q) && \text{by the first De Morgan law}\\
		&\equiv (p \vee q) \wedge (\neg p \vee \neg q) && \text{by commutative law}
	\end{align*}
\end{center}
\endgroup
\section*{Q. 2}

\begin{center}
	\begin{align*}
		&\textbf{a.  } \forall x \forall y \forall f ((I(x, f) \wedge I(y, f)) \rightarrow \neg \exists z(E(x, z) \wedge E(y, z))) \\
		&\textbf{b.  } \forall f \exists x (I(x, f) \wedge S(x,x) \wedge \neg \exists y (S(x, y) \wedge y \neq x))\\
		&\textbf{c.  } \forall j (J(j, m) \rightarrow \exists x \exists y ((A(x, j) \wedge A(y, j) \wedge x \neq y) \rightarrow \neg \exists z (A(z, j) \wedge z \neq x \wedge z \neq y)))\\ 
		&\text{Note: $m$ is constant and means medicine faculty}
	\end{align*}
\end{center}

\section*{Q. 3}

\begin{center}
	\textbf{a.  } 
	\begin{fitchproof}
		\fitchline{$p \vee \neg q$}{premise}
		\fitchline{$p \vee r$}{premise}
		\subproof{
			\fitchline{$ r \rightarrow q $}{assumption}
			\subproof{
				\fitchline{$ \neg p $}{assumption}
				\subproof{
					\fitchline{$p$}{assumption}
					\fitchline{$\bot$}{$\neg e$ 4,5}
					\fitchline{$r$}{$\bot e$ 4}
					\fitchline{$\neg q$}{$\bot e$ 4}
				}
				
				\subproof{
					\fitchline{$r$}{assumption}
				}
				
				\subproof{
					\fitchline{$\neg q$}{assumption}
				}
			
				\fitchline{$r$}{$\vee e$ 5--7, 9}
				\fitchline{$\neg q$}{$\vee e$ 5--8, 10}
				\fitchline{$q$}{$\rightarrow e$ 3,11}
				\fitchline{$\bot$}{$\neg e$ 12,13}
			}
			\fitchline{$\neg \neg p$}{$\neg i$ 4--14}
			\fitchline{$p$}{$\neg \neg e$ 15}
		}
		\fitchline{$(r \rightarrow q) \rightarrow p$}{$\rightarrow i$ 3--16}
		
	\end{fitchproof}

	\textbf{b.  } 
	\begin{fitchproof}
		\subproof{
			\fitchline{$((q \rightarrow p) \rightarrow q)$}{assumption}
			\subproof{
				\fitchline{$\neg q$}{assumption}
				\subproof{
					\fitchline{$q \rightarrow p$}{assumption}
					\fitchline{$q$}{$\rightarrow e$ 1,3}
					\fitchline{$\bot$}{$\neg e$ 2,4}
				}
				\fitchline{$\neg (q \rightarrow p)$}{$\neg i$ 3--5}
				\fitchline{$\neg(\neg q \vee p)$}{derived proof (3)}
				\fitchline{$\neg \neg q \wedge \neg p$}{derived proof (2)}
				\fitchline{$q \wedge \neg p$}{$\neg \neg e$ 8}
				\fitchline{$q$}{$\wedge e$ 9}
				\fitchline{$\bot$}{$\neg e$ 2,10}
			}
			\fitchline{$\neg \neg q$}{$\neg i$ 2--11}
			\fitchline{$q$}{$\neg \neg e$ 12}
		}
		\fitchline{$((q \rightarrow p) \rightarrow q) \rightarrow q$}{$\rightarrow i$ 1--13}
	\end{fitchproof}
\end{center}

\section*{Q. 4}

\begin{center}
	\textbf{a.  } 
	\begin{fitchproof}
		\fitchline{$\neg \forall x (P(x) \rightarrow Q(x))$}{premise}
		\fitchline{$\neg (P(a) \rightarrow Q(x))$}{$\forall e$ 1}
		\fitchline{$\neg (\neg P(a) \vee Q(a))$}{derived proof (3)}
		\fitchline{$\neg \neg P(a) \wedge \neg Q(a)$}{derived proof (2)}
		\fitchline{$P(a) \wedge \neg Q(a)$}{$\neg \neg e$ 4}
		\fitchline{$\exists x (P(x) \wedge \neg Q(x))$}{$\exists i$ 1--5}
	\end{fitchproof}
\end{center}

\section*{Derived Proofs}

\begin{center}
	\begin{equation}
		\neg (p \wedge q) \vdash \neg p \vee \neg q.
	\end{equation}
	\begin{fitchproof}
		\fitchline{$\neg (p \wedge q)$}{premise}
		\subproof{
			\fitchline{$\neg (\neg p \vee \neg q)$}{assumption}
			\subproof{
				\fitchline{$ \neg p$}{assumption}
				\fitchline{$\neg p \vee \neg q$}{$\vee i$ 3}
				\fitchline{$\bot$}{$\neg e$ 2,4}
			}
			\fitchline{$\neg \neg p$}{$\neg i$ 3--5}
			\fitchline{$p$}{$\neg \neg e$ 6}
			\subproof{
				\fitchline{$\neg q$}{assumption}
				\fitchline{$\neg p \vee \neg q$}{$\vee i$ 8}
				\fitchline{$\bot$}{$\neg e$ 2,9}
			}
			\fitchline{$\neg \neg q$}{$\neg i$ 8--10}
			\fitchline{$q$}{$\neg \neg i$ 11}
			\fitchline{$p \wedge q$}{$\wedge i$ 7,12}
			\fitchline{$\bot$}{$\neg e$ 1,13}
		}
		\fitchline{$\neg p \vee \neg q$}{$\neg i$ 1,14}
	\end{fitchproof}
\end{center}

\begin{center}
	\begin{equation}
		\neg (p \vee q) \vdash \neg p \wedge \neg q.
	\end{equation}
	\begin{fitchproof}
		\fitchline{$\neg (p \vee q)$}{premise}
		\subproof{
			\fitchline{$\neg (\neg p \wedge \neg q)$}{assumption}
			\fitchline{$\neg \neg p \vee \neg \neg q$}{derived proof (1)}
			\fitchline{$p \vee q$}{$\neg \neg e$ 3}
			\fitchline{$\bot$}{$\neg e$ 1,4}
		}
		\fitchline{$\neg p \wedge \neg q$}{$\neg i$ 2--5}
	\end{fitchproof}
\end{center}

\begin{center}
	\begin{equation}
		p \rightarrow q \vdash \neg p \vee q.
	\end{equation}
	\begin{fitchproof}
		\fitchline{$p \rightarrow q$}{premise}
		\subproof{
			\fitchline{$\neg (\neg p \vee q)$}{assumption}
			\fitchline{$\neg \neg p \wedge \neg q$}{derived proof (2)}
			\fitchline{$p \wedge \neg q$}{$\neg \neg e$ 3}
			\fitchline{$p$}{$\wedge e$ 4}
			\fitchline{$\neg q$}{$\wedge e$ 4}
			\fitchline{$q$}{$\rightarrow e$ 1,5}
			\fitchline{$\bot$}{$\neg e$ 6,7}
		}
		\fitchline{$\neg \neg (\neg p \vee q)$}{$\neg e$ 2--8}
		\fitchline{$\neg p \vee q$}{$\neg \neg e$ 9}
	\end{fitchproof}
\end{center}

% add / remove sections etc as needed 
% use your own format

\end{document}

